NuSys.thy
@@ -62,11 +62,11 @@ ML_file NuHelp.ML
 
 subsection \<open>Code Block & Current Construction & Pending Construction\<close>
 
-definition (in std) CodeBlock :: "('VAL,'RES_N,'RES) state
-                               \<Rightarrow> ('VAL,'RES_N,'RES) state
-                               \<Rightarrow> ('VAL,'RES_N,'RES) proc
-                               \<Rightarrow> ('VAL,'FIC_N,'FIC) assn
-                               \<Rightarrow> ('VAL,'FIC_N,'FIC) assn
+definition (in std) CodeBlock :: "('RES_N \<Rightarrow> 'RES)
+                               \<Rightarrow> ('RES_N \<Rightarrow> 'RES)
+                               \<Rightarrow> ('VAL,'RES_N,'RES) M
+                               \<Rightarrow> ('FIC_N,'FIC) assn
+                               \<Rightarrow> ('FIC_N,'FIC) assn
                                \<Rightarrow> bool"
   where "CodeBlock stat arg prog R E \<longleftrightarrow>
              (bind arg prog = stat \<and> stat \<noteq> PartialCorrect \<and> (\<forall>s \<in> INTERP_COMP (R * E). stat \<noteq> Exception s))"
@@ -75,23 +75,25 @@ definition (in std) CodeBlock :: "('VAL,'RES_N,'RES) state
 syntax "_codeblock_" :: "idt \<Rightarrow> logic \<Rightarrow> bool" ("\<^bold>c\<^bold>o\<^bold>d\<^bold>e\<^bold>b\<^bold>l\<^bold>o\<^bold>c\<^bold>k _ \<^bold>f\<^bold>o\<^bold>r \<^bold>a\<^bold>r\<^bold>g\<^bold>u\<^bold>m\<^bold>e\<^bold>n\<^bold>t\<^bold>s '\<open>_'\<close>" [100,0] 3) *)
 
 definition (in std)
-  CurrentConstruction :: " ('VAL,'RES_N,'RES) state
-                        \<Rightarrow> ('VAL,'FIC_N,'FIC) assn
-                        \<Rightarrow> ('VAL,'FIC_N,'FIC) assn \<Rightarrow> bool "
+  CurrentConstruction :: " ('RES_N \<Rightarrow> 'RES)
+                        \<Rightarrow> ('FIC_N,'FIC) assn
+                        \<Rightarrow> ('FIC_N,'FIC) assn \<Rightarrow> bool "
     ("\<^bold>c\<^bold>u\<^bold>r\<^bold>r\<^bold>e\<^bold>n\<^bold>t _ [_]/ \<^bold>r\<^bold>e\<^bold>s\<^bold>u\<^bold>l\<^bold>t\<^bold>s \<^bold>i\<^bold>n _" [1000,1000,11] 10)
-  where "CurrentConstruction s R S \<longleftrightarrow> s \<in> !\<S> (INTERP_COMP (R * S)) {}"
+  where "CurrentConstruction s R S \<longleftrightarrow> s \<in> (INTERP_COMP (R * S))"
+
+term bind
 
 definition (in std)
   PendingConstruction :: " ('VAL,'RES_N,'RES) proc
-                        \<Rightarrow> ('VAL,'RES_N,'RES) state
-                        \<Rightarrow> ('VAL,'FIC_N,'FIC) assn
-                        \<Rightarrow> ('VAL,'FIC_N,'FIC) assn
-                        \<Rightarrow> ('VAL,'FIC_N,'FIC) assn \<Rightarrow> bool "
+                        \<Rightarrow> ('RES_N \<Rightarrow> 'RES)
+                        \<Rightarrow> ('FIC_N,'FIC) assn
+                        \<Rightarrow> ('VAL list \<Rightarrow> ('FIC_N,'FIC) assn)
+                        \<Rightarrow> ('FIC_N,'FIC) assn \<Rightarrow> bool "
     ("\<^bold>p\<^bold>e\<^bold>n\<^bold>d\<^bold>i\<^bold>n\<^bold>g _ \<^bold>o\<^bold>n _ [_]/ \<^bold>r\<^bold>e\<^bold>s\<^bold>u\<^bold>l\<^bold>t\<^bold>s \<^bold>i\<^bold>n _/ \<^bold>t\<^bold>h\<^bold>r\<^bold>o\<^bold>w\<^bold>s _" [1000,1000,1000,11,11] 10)
-    where "PendingConstruction f s R S E \<longleftrightarrow> bind s f \<in> \<S> (INTERP_COMP (R * S)) (INTERP_COMP (R * E))"
+    where "PendingConstruction f s R S E \<longleftrightarrow> f s \<in> \<S> (\<lambda>ret. INTERP_COMP (R * S ret)) (INTERP_COMP (R * E))"
 
 lemma (in std) CurrentConstruction_D: "CurrentConstruction s H T \<Longrightarrow> Inhabited T"
-  unfolding CurrentConstruction_def Inhabited_def by (cases s) (auto 0 4 simp add: \<phi>expns)
+  unfolding CurrentConstruction_def Inhabited_def by (auto 0 4 simp add: \<phi>expns)
 
 lemma (in std) CurrentConstruction_mk_elim_rule:
   "CurrentConstruction s H T \<Longrightarrow> (Inhabited T \<Longrightarrow> C) \<Longrightarrow> C"
@@ -101,7 +103,7 @@ lemma (in std) CurrentConstruction_mk_elim_rule:
 
 paragraph \<open>Rules for Constructing Programs\<close>
 
-definition \<open>EMPTY_PROC = SKIP\<close>
+definition \<open>EMPTY_PROC = Success\<close>
 
 context std begin
 
